x86/RawAsm.v
@@ -24,12 +24,18 @@ Section WITHMEMORYMODEL.
 Section WITHGE.
   Variable ge : Genv.t Asm.fundef unit.
 
+  Definition maybe_storev chunk m addr v : option mem :=
+    match Mem.loadv chunk m addr with
+    | Some v' => if Val.eq v v' then Some m else Mem.storev chunk m addr v
+    | None => None
+    end.
+  
   Definition exec_instr f i rs (m: mem) :=
     let isz := Ptrofs.repr (Asm.instr_size i) in
     match i with
     | Pallocframe fi ofs_ra =>
       let sp := Val.offset_ptr (rs RSP) (Ptrofs.neg (Ptrofs.repr (align (frame_size fi) 8))) in
-      match Mem.storev Mptr m (Val.offset_ptr sp ofs_ra) rs#RA with
+      match maybe_storev Mptr m (Val.offset_ptr sp ofs_ra) rs#RA with
       | None => Stuck
       | Some m2 =>
         Next (nextinstr (rs #RAX <- (rs#RSP) #RSP <- sp) isz) m2
@@ -84,10 +90,11 @@ Section WITHGE.
           (RA_TYPE: Val.has_type (rs RA) Tptr)
           (SP_NOT_VUNDEF: rs RSP <> Vundef)
           (RA_NOT_VUNDEF: rs RA <> Vundef)
-          (SZRA: Mem.storev Mptr m (Val.offset_ptr (rs RSP) (Ptrofs.neg (Ptrofs.repr (size_chunk Mptr))))
+          (SZRA: maybe_storev Mptr m (Val.offset_ptr (rs RSP) (Ptrofs.neg (Ptrofs.repr (size_chunk Mptr))))
                             (rs RA) = Some m2)
           (ARGS: extcall_arguments rs m2 (ef_sig ef) args),
           external_call ef ge args m2 t res m' ->
+          ra_after_call ge (rs#RA) ->
           rs' = (set_pair (loc_external_result (ef_sig ef)) res (undef_regs (CR ZF :: CR CF :: CR PF :: CR SF :: CR OF :: nil) (undef_regs (map preg_of destroyed_at_call) rs))) #PC <- (rs RA) #RA <- Vundef ->
           step (State rs m) t (State rs' m').
 
@@ -153,7 +160,7 @@ Section WITHMEMORYMODEL2.
         exploit Events.external_call_determ. eexact H5. eexact H11. intros [A B].
         split. auto. intros. destruct B; auto. subst. auto.
       + assert (args0 = args) by (eapply Asm.extcall_arguments_determ; eauto). subst args0.
-        exploit Events.external_call_determ. eexact H3. eexact H7. intros [A B].
+        exploit Events.external_call_determ. eexact H3. eexact H8. intros [A B].
         split. auto. intros. destruct B; auto. subst. auto.
     - (* trace length *)
       red; intros; inv H; simpl.
@@ -188,7 +195,7 @@ Section WITHMEMORYMODEL2.
         exploit Events.external_call_determ. eexact H5. eexact H11. intros [A B].
         split. auto. intros. destruct B; auto. subst. auto.
       + assert (args0 = args) by (eapply Asm.extcall_arguments_determ; eauto). subst args0.
-        exploit Events.external_call_determ. eexact H3. eexact H7. intros [A B].
+        exploit Events.external_call_determ. eexact H3. eexact H8. intros [A B].
         split. auto. intros. destruct B; auto. subst. auto.
     - (* trace length *)
       red; intros; inv H; simpl.
